Clike spec and abstract spec equivalence proof sketch

src/C_strtoimax/VstProof/AbstractSpec.v
@@ -88,6 +88,115 @@ Section AbstractSpec.
 
 End AbstractSpec.
 
+Section ClikeSpec.
+
+Definition ASN1_INTMAX_MAX := Int64.max_signed.
+Definition upper_boundary := Z.div ASN1_INTMAX_MAX 10.
+Definition last_digit_max := Zmod ASN1_INTMAX_MAX 10.
+Definition last_digit_max_minus := last_digit_max + 1.
+
+Definition app_char (b : bool) v c := 
+  if b then  v * 10 + (Z_of_char c) else -v * 10 - (Z_of_char c).
+
+Definition last_digit (b : bool) := 
+  if b then last_digit_max else last_digit_max_minus.
+
+Fixpoint Z_of_string_loop_C (s : list byte) (v i : Z) (b : bool):= 
+    match s with 
+    | [] => {| res := OK ; 
+              value := v ; 
+              index := i |}
+    | c :: tl => 
+      if is_digit c
+      then let d := (Z_of_char c) in 
+           if (v <? upper_boundary) 
+           then Z_of_string_loop_C tl (v * 10 + d) (i + 1) b
+           else if ((v =? upper_boundary)&&(d <=? (last_digit b)))%bool
+                then let v1 := app_char b v c in
+                     match tl with
+                     | [] => {| res := OK ; 
+                               value := v1 ; 
+                               index := (i + 1) |}
+                     | c :: tl => if is_digit c
+                                 then {| res := ERROR_RANGE ;
+                                         value := v1;
+                                         index := (i + 1) ; |}
+                                 else {| res := EXTRA_DATA;
+                                         value := v1 ;
+                                         index := (i + 1) ; |}
+                     end
+                else {| res := ERROR_RANGE ;
+                        value := v ;
+                        index := i ; |}      
+      else {| res := EXTRA_DATA ;
+              value := v ;
+              index := i ; |}              
+    end.
+
+Definition Z_of_string_C (s : list byte) : Z_of_string_result := 
+  match s with 
+  |  nil => {| res := ERROR_INVAL ; 
+              value := 0 ;
+              index := 0 ; |} 
+  | [ch] => if is_sign ch 
+           then {| res := EXPECT_MORE ;
+                   value := 0 ;
+                   index := 1 ; |} 
+           else Z_of_string_loop_C s 0 0 true
+  |  ch :: tl => let result := Z_of_string_loop_C tl 0 1 true in
+               if (Byte.signed ch =? plus_char)
+               then result
+               else if (Byte.signed ch =? minus_char)
+                    then let v := value (Z_of_string_loop_C tl 0 1 false) in 
+                         {| res := res result ;
+                            value := if 0 <? v then (-1*v) else v  ;
+                            index := index result ; |}
+                    else Z_of_string_loop_C s 0 0 true
+  end.
+
+End ClikeSpec.
+
+Section AbstractSpec''.
+
+ Fixpoint Z_of_string_loop'' (s : list byte) (v i : Z) (b : bool) := 
+    match s with 
+    | [] => {| res := OK ; 
+              value := v ; 
+              index := i |}
+    | c :: tl => 
+      if is_digit c
+      then let v1 := app_char b v c in 
+           if bounded v1
+           then Z_of_string_loop'' tl v1 (i + 1) b
+           else {| res := ERROR_RANGE ;
+                   value := v ;
+                   index := i ; |}      
+      else {| res := EXTRA_DATA ;
+              value := v ;
+              index := i ; |}              
+    end.
+
+
+  Definition Z_of_string'' (s : list byte) : Z_of_string_result := 
+      match s with 
+      |  nil => {| res := ERROR_INVAL ; 
+                  value := 0 ;
+                  index := 0 ; |} 
+      | [ch] => if is_sign ch 
+                then {| res := EXPECT_MORE ;
+                        value := 0 ;
+                        index := 1 ; |} 
+                else Z_of_string_loop'' s 0 0 true
+      |  ch :: tl => if (Byte.signed ch =? plus_char)
+                    then  Z_of_string_loop'' tl 0 1 true
+                    else if (Byte.signed ch =? minus_char)
+                         then Z_of_string_loop'' tl 0 1 false
+                         else Z_of_string_loop'' s 0 0 true
+      end.
+
+End AbstractSpec''.
+
+
 Section AbstractSpec'.
 
   (* true plus, false minus bound *)
@@ -107,7 +216,7 @@ Section AbstractSpec'.
            if bounded' b v1
            then Z_of_string_loop' tl v1 (i + 1) b
            else {| res := ERROR_RANGE ;
-                   value := v1 ;
+                   value := v ;
                    index := i ; |}      
       else {| res := EXTRA_DATA ;
               value := v ;
@@ -136,3 +245,193 @@ Section AbstractSpec'.
       end.
 
 End AbstractSpec'.
+
+Lemma aux : forall ls v i, Z_of_string_loop'' ls v i true = 
+                      Z_of_string_loop_C ls v i true.
+  Proof.
+    induction ls.
+    - intuition.
+    - simpl.
+      intros.
+      repeat break_if;
+        try eapply IHls.
+      break_match.
+      -- intuition.
+      -- break_if.
+         simpl.
+         bool_rewrite.
+         break_if.
+         (* contrdiction *)
+         admit.
+         intuition.
+         simpl.
+         bool_rewrite.
+         intuition.
+      --(* contradiction *)
+        admit.
+      -- (* contradiction *)
+        admit.
+      -- break_match.
+         * (* contradiction *)
+           admit.
+         * (* contradiction *)
+           admit.
+Admitted.
+
+
+Lemma aux' : forall ls v i, Z_of_string_loop' ls v i true = 
+                      Z_of_string_loop_C ls v i true.
+  Proof.
+    induction ls.
+    - intuition.
+    - simpl.
+      intros.
+      repeat break_if;
+        try eapply IHls.
+      break_match.
+      -- intuition.
+      -- break_if.
+         simpl.
+         bool_rewrite.
+         break_if.
+         (* contrdiction *)
+         admit.
+         intuition.
+         simpl.
+         bool_rewrite.
+         intuition.
+      -- (* contradiction *)
+        admit.
+      -- (* contradiction *)
+        admit.
+      -- break_match.
+         * (* contradiction *)
+           admit.
+         * (* contradiction *)
+           admit.
+Admitted.
+
+Ltac Zbool_to_Prop := try (rewrite Z.leb_le ||
+                           rewrite Z.leb_gt ||
+                           rewrite Z.eqb_eq ||
+                           rewrite Z.eqb_neq).
+
+Lemma is_digit_to_Z : forall c, is_digit c = true -> 0 <= Z_of_char c <= 9.
+Proof.
+  unfold is_digit, Z_of_char.
+  intro.
+  rewrite andb_true_iff in *.
+  repeat Zbool_to_Prop.
+  unfold zero_char, nine_char.
+  nia.
+Qed.
+
+Lemma loop_non_neg : forall ls v i, 0 <= v -> 0 <= value (Z_of_string_loop' ls v i false).
+Proof.
+  induction ls.
+  - intuition.
+  - intros.
+    simpl.
+      repeat break_if;
+    simpl; try congruence;
+       eapply is_digit_to_Z in Heqb.
+    eapply IHls.
+    all: nia.
+Qed.
+
+
+  Lemma aux_false : forall ls v i, 
+      0 <= v ->
+      0 <= value (Z_of_string_loop' ls v i false) ->
+      value (Z_of_string_loop' ls v i false) = 
+      Z.abs (value (Z_of_string_loop_C ls v i false)).
+  Proof.
+    induction ls.
+    - simpl.
+      intros.
+      auto with zarith.
+      erewrite Z.abs_eq;
+        try nia.
+    - simpl.
+      intros.
+      repeat break_if;
+        try eapply IHls.
+       eapply is_digit_to_Z in Heqb.
+       nia.
+      eapply loop_non_neg.
+        eapply is_digit_to_Z in Heqb.
+       nia.
+      break_match.
+      -- simpl. 
+         assert (0 <= v * 10 + Z_of_char a).
+         eapply is_digit_to_Z in Heqb.
+         nia.
+         replace (- v * 10 - Z_of_char a) with
+           (- (v * 10 + Z_of_char a))
+                 by auto with zarith.
+          Search Z.abs Z.opp.
+          erewrite Z.abs_opp.
+          edestruct  Z.abs_spec with (n :=  v * 10 + Z_of_char a).
+          inversion H2.
+          nia.
+          inversion H2.
+          nia.
+      -- break_if.
+         simpl.
+         bool_rewrite.
+         break_if.
+         (* contrdiction *)
+         admit.
+         admit.
+         simpl.
+         bool_rewrite.
+         simpl.
+          assert (0 <= v * 10 + Z_of_char a).
+         eapply is_digit_to_Z in Heqb.
+         nia.
+         replace (- v * 10 - Z_of_char a) with
+           (- (v * 10 + Z_of_char a))
+                 by auto with zarith.
+          Search Z.abs Z.opp.
+          erewrite Z.abs_opp.
+          edestruct  Z.abs_spec with (n :=  v * 10 + Z_of_char a).
+          inversion H2.
+          nia.
+          inversion H2.
+          nia.
+      -- (* contradiction *)
+        admit.
+      -- (* contradiction *)
+        admit.
+      --  (* contradiction *)
+        admit.
+Admitted. 
+
+Lemma Clike_corr : forall ls, Z_of_string' ls = Z_of_string_C ls.
+  Proof.
+    destruct ls.
+    - intuition.
+    - simpl.
+      repeat break_if;
+        try congruence; try eapply aux'.
+        simpl. (* contradiction *) admit.
+        replace (Z_of_string_loop_C (i0 :: l) 0 1 true) with
+            (Z_of_string_loop' (i0 :: l) 0 1 true).
+        replace (value (Z_of_string_loop' (i0 :: l) 0 1 false))
+                with (Z.abs (value (Z_of_string_loop_C (i0 :: l) 0 1 false))).
+        admit.
+        erewrite  aux_false.
+        auto.
+        nia.
+        admit.
+        eapply aux'.
+        erewrite aux_false.
+        admit.
+        nia.
+        admit.
+        admit.
+Admitted.
+                
+
+      
+  
